learnings/remember.md
@@ -1,0 +1,29 @@
+# remember
+
+In Coq we first used the `remember` tactic to first create an hyptohesis for the comparison and then did case analysis on the comparison. Lean has a shorthand for this as part of the cases tatic.
+
+There might be other alternative options, but if we think specifically the use case of breaking up a hypothesis on `compare` with `cases` there is shorthand that is very helpful.
+
+> cases h : e, where e is a variable or an expression, performs cases on e as above, but also adds a hypothesis h : e = ... to each hypothesis, where ... is the constructor instance for that particular case.
+
+```lean
+def compare_isle_is_decidable {α: Type u} (x y: α) [o: Ord α]: Decidable (Ord.compare x y).isLE := by
+  unfold isLE
+  cases h: compare x y
+  · case lt =>
+    simp only
+    apply Decidable.isTrue
+    simp only
+  · case eq =>
+    simp only
+    apply Decidable.isTrue
+    simp only
+  · case gt =>
+    simp only
+    apply Decidable.isFalse
+    simp only [Bool.false_eq_true, not_false_eq_true]
+```
+
+## References
+
+* [cases tactic](https://github.com/haruhisa-enomoto/mathlib4-all-tactics/blob/main/all-tactics.md#cases)
